coq/SimpleForm/Interpretation.v
@@ -495,7 +495,7 @@ Section Interpretation.
         apply var_in_sact_ok_inv. apply H. unfold var_lt. lia.
   Qed.
 
-  Definition useful_vars (sf: simple_form (reg_t:=reg_t) (ext_fn_t:=ext_fn_t))
+  Definition useful_vars (sf: simple_form (reg_t:=reg_t) (ext_fn_t:=ext_fn_t) (rule_name_t := rule_name_t))
   : list positive :=
     let todo := map snd (final_values sf) in
     fold_left
@@ -555,7 +555,7 @@ Section Interpretation.
     eapply useful_vars_incl; eauto.
   Qed.
 
-  Definition simple_form := simple_form (reg_t:=reg_t) (ext_fn_t:=ext_fn_t).
+  Definition simple_form := simple_form (reg_t:=reg_t) (ext_fn_t:=ext_fn_t) (rule_name_t := rule_name_t).
 
   Fixpoint eval_sact (vars: var_value_map) (a: sact) (fuel: nat) : option val :=
     match fuel with
