coq/SimpleForm/Simplifications/Collapse.v
@@ -25,7 +25,7 @@ Section Collapse.
   Context (sigma: ext_funs_defs).
   Local Definition sact := sact (ext_fn_t := ext_fn_t) (reg_t := reg_t).
   Local Definition eval_sact := eval_sact r sigma.
-  Local Definition wf_sf := wf_sf R Sigma.
+  Local Definition wf_sf := wf_sf (rule_name_t := rule_name_t) R Sigma.
   Hypothesis WTRENV: Wt.wt_renv R REnv r.
   Context {
     wt_sigma:
@@ -56,7 +56,7 @@ Section Collapse.
     end.
 
   (* Note that *)
-  Definition collapse_sf (sf: simple_form) :=
+  Definition collapse_sf (sf: simple_form (rule_name_t := rule_name_t)) :=
     sf <| vars :=
       (* TODO Alternatively, fold and handle elements in order. That would
          remove the need for successive calls to collapse. *)
